delete not used functions [2]

code/experimental/P256/Hacl.Spec.P256.MontgomeryMultiplication.fst
@@ -4,67 +4,50 @@ open FStar.Math.Lemmas
 open FStar.Math.Lib
 open FStar.Mul
 
-open FStar.HyperStack.All
-open FStar.HyperStack
-open FStar.HyperStack.ST
-module ST = FStar.HyperStack.ST
-
 open Hacl.Spec.P256.Lemmas
 open Hacl.Spec.P256.Definitions
 open Hacl.Spec.P256.Core
 
 open Lib.IntTypes
-open Lib.Buffer
-open Lib.Sequence
-open Lib.Loops
 
-#reset-options "--z3rlimit 300"
+#set-options "--z3rlimit 300"
 
 let prime = prime256
 
+
 let fromDomain_ a = (a * modp_inv2 (pow2 256)) % prime256
+
 
 let fromDomainPoint a = 
   let x, y, z = a in 
   fromDomain_ x, fromDomain_ y, fromDomain_ z
 
 
-val fromDomain: a: felem4{as_nat4 a < prime256} -> Tot (result: felem4 {as_nat4 result = fromDomain_ (as_nat4 a)})
-
-let fromDomain a =  
-  let one = ((u64 1), (u64 0), u64 0, u64 0) in
-    assert_norm (as_nat4 one = 1);
-  Core.montgomery_multiplication one a
-
-
 let toDomain_ a = (a * pow2 256) % prime256
 
+
 let lemmaFromDomain a = ()
+
 
 let lemmaToDomain a = ()
 
 
-#reset-options "--z3rlimit 300 --z3refresh"
-
 let lemmaToDomainAndBackIsTheSame a = 
   let to = toDomain_ a in 
-    lemmaToDomain a;
+  lemmaToDomain a;
   let from = fromDomain_ to in 
-    lemmaFromDomain to;
-    lemma_mod_mul_distr_l (a * pow2 256) (modp_inv2 (pow2 256)) prime256;
-    assert(from = (a * pow2 256 * modp_inv2 (pow2 256)) % prime256);
-    assert_norm (pow2 256 * modp_inv2 (pow2 256) % prime256 = 1);
+  lemmaFromDomain to;
+  lemma_mod_mul_distr_l (a * pow2 256) (modp_inv2 (pow2 256)) prime256;
+  assert_norm (pow2 256 * modp_inv2 (pow2 256) % prime256 = 1);
   modulo_distributivity_mult_last_two a 1 1 (pow2 256) (modp_inv2 (pow2 256)) prime256;
-    assert((a * pow2 256 * modp_inv2 (pow2 256)) % prime256 == (a * (pow2 256 * modp_inv2 (pow2 256) % prime)) % prime256);
-    modulo_lemma a prime;
-    assert(from = a)
+  modulo_lemma a prime
 
 
 let lemmaFromDomainToDomain a = 
   let from = fromDomain_ a in 
-    lemmaFromDomain a;
+  lemmaFromDomain a;
   let to = toDomain_ from in 
-    lemmaToDomain from;
+  lemmaToDomain from;
   lemma_mod_mul_distr_l (a * modp_inv2 (pow2 256)) (pow2 256)  prime256;
   assert_norm (modp_inv2 (pow2 256) * (pow2 256) % prime = 1);
   modulo_distributivity_mult_last_two a 1 1 (modp_inv2 (pow2 256)) (pow2 256) prime256;
@@ -76,109 +59,36 @@ let lemmaFromDomainToDomainModuloPrime a =
   assert_norm (pow2 256 * modp_inv2 (pow2 256) % prime256 = 1);
   modulo_distributivity_mult_last_two a 1 1 (pow2 256) (modp_inv2 (pow2 256)) prime256
 
-(* it is the key lemma of Montgomery Multiplication, showing that it's correct (i.e. mm(a, b) = a * b * 2^-256 *)
-(*
-val lemmaMontgomeryMultiplicationCorrect: a: felem4{as_nat4 a < prime} -> b: felem4{as_nat4 b < prime} -> Lemma (
-  let aDomain = toDomain_ a in 
-  let bDomain = toDomain b in 
-  let multInDomain = Core.montgomery_multiplication aDomain bDomain in 
-  let multResultFromDomain = fromDomain multInDomain in 
-  as_nat4 a * as_nat4 b % prime == as_nat4 multResultFromDomain)
-
-
-let lemmaMontgomeryMultiplicationCorrect a b = 
-  let aDomain = toDomain a in 
-  let bDomain = toDomain b in 
-  let multInDomain = montgomery_multiplication aDomain bDomain in 
-  assert_norm (prime > 0);
-  modulo_distributivity_mult2 (as_nat4 a * pow2 256) (as_nat4 b * pow2 256) (modp_inv2 (pow2 256)) prime;  
-  lemma_brackets_l (as_nat4 a * pow2 256) ((as_nat4 b * pow2 256) * modp_inv2 (pow2 256)) (modp_inv2 (pow2 256));
-  lemma_twice_brackets (as_nat4 a) (pow2 256) 1 (as_nat4 b) (pow2 256) 1 (modp_inv2 (pow2 256));
-  modulo_distributivity_mult2 (as_nat4 a * pow2 256) (as_nat4 b * pow2 256) (modp_inv2 (pow2 256)) prime;
-  modulo_distributivity_mult_last_two (as_nat4 a) (pow2 256) (as_nat4 b) (pow2 256) (modp_inv2 (pow2 256)) prime;
-  assert_norm((pow2 256 * modp_inv2 (pow2 256)) % prime = 1);
-  lemma_distr_mult3 (as_nat4 a) (pow2 256) (as_nat4 b);
-  let multFromDomain = fromDomain multInDomain in 
-  lemma_mod_mul_distr_l (as_nat4 a * as_nat4 b *pow2 256) (modp_inv2 (pow2 256)) prime;
-  modulo_distributivity_mult_last_two (as_nat4 a) (as_nat4 b) 1 (pow2 256) (modp_inv2 (pow2 256)) prime
-*)
-
 
 let inDomain_mod_is_not_mod a = 
   lemma_mod_mul_distr_l a (pow2 256) prime256
-
-
-(* the lemma shows that the result of multiplication moved out of domain is the multiplication of the numbers moved out of domain *)
-val multiplicationInDomain: #k: nat -> #l: nat -> 
-  a: felem4 {as_nat4 a == toDomain_ (k) /\ as_nat4 a < prime} -> 
-  b: felem4 {as_nat4 b == toDomain_ (l) /\ as_nat4 b < prime256} -> Lemma 
-    (ensures (let multResult = Core.montgomery_multiplication a b in as_nat4 multResult == toDomain_ (k * l)))
-    
-let multiplicationInDomain #k #l a b = 
-  let multResult = Core.montgomery_multiplication a b in 
-  lemma_mul_nat2 k l;
-  let secondBracket = toDomain_ (k * l) in 
-    assert(as_nat4 multResult = toDomain_ (k) * toDomain_ (l) * modp_inv2 (pow2 256) % prime);
-  modulo_distributivity_mult2 (k * pow2 256) (l* pow2 256) (modp_inv2 (pow2 256)) prime;
-  lemma_twice_brackets k (pow2 256) 1 l (pow2 256) 1 (modp_inv2 (pow2 256));
-  assert_norm (pow2 256 * modp_inv2 (pow2 256) % prime == 1);
-  modulo_distributivity_mult_last_two k (pow2 256) l (pow2 256) (modp_inv2 (pow2 256)) prime;
-  lemma_mul_ass3 k (pow2 256) l
 
 
 let multiplicationInDomainNat #k #l a b = 
   assert_norm (prime256 > 3);
   let multResult = a * b * modp_inv2_prime (pow2 256) prime256 % prime256 in 
   modulo_distributivity_mult2 (k * pow2 256) (l * pow2 256) (modp_inv2_prime (pow2 256) prime256) prime;
-   lemma_twice_brackets k (pow2 256) 1 l (pow2 256) 1 (modp_inv2 (pow2 256));
+  lemma_twice_brackets k (pow2 256) 1 l (pow2 256) 1 (modp_inv2 (pow2 256));
   assert_norm (pow2 256 * modp_inv2 (pow2 256) % prime == 1);
   modulo_distributivity_mult_last_two k (pow2 256) l (pow2 256) (modp_inv2 (pow2 256)) prime;
   lemma_mul_ass3 k (pow2 256) l
 
 
-val additionInDomain: #k: nat -> #l: nat -> 
-  a: felem4 {as_nat4 a == toDomain_ (k) /\ as_nat4 a < prime} -> 
-  b: felem4 {as_nat4 b == toDomain_ (l) /\ as_nat4 b < prime} -> Lemma 
-  (ensures (let result = felem_add a b in as_nat4 result == toDomain_(k + l)))
-
-let additionInDomain #k #l a b = 
-  let result = felem_add a b in 
-  assert(as_nat4 result = (as_nat4 a + as_nat4 b) % prime);
-  assert(as_nat4 result = (toDomain_(k) + toDomain_(l)) % prime);
-  assert(as_nat4 result = ((k * pow2 256 % prime) + (l * pow2 256 % prime)) % prime);
-  modulo_distributivity (k * pow2 256) (l *pow2 256) prime;
-  assert(as_nat4 result = toDomain_ (k + l))
-
-
-val additionInDomainNat: #k: nat -> #l: nat -> a: nat {a == toDomain_ k /\ a < prime} -> b: nat {b == toDomain_ l /\ b < prime} ->
-  Lemma (let result = (a + b) % prime in result == toDomain_ (k + l))
-
-let additionInDomainNat #k #l a b = 
+let additionInDomain a b = 
+  let k = fromDomain_ a in 
+  let l = fromDomain_ b in 
+  lemmaFromDomainToDomain a;
+  lemmaFromDomainToDomain b;
   modulo_distributivity (k * pow2 256) (l * pow2 256) prime
 
 
-let additionInDomain2Nat a b = 
+let substractionInDomain a b = 
   let k = fromDomain_ a in 
   let l = fromDomain_ b in 
   lemmaFromDomainToDomain a;
   lemmaFromDomainToDomain b;
-  additionInDomainNat #k #l a b
-
-
-val substractionInDomainNat: #k: nat -> #l: nat -> a: nat {a == toDomain_ k /\ a < prime} -> b: nat {b == toDomain_ l /\ b < prime} -> 
-  Lemma ((a - b) % prime  == toDomain_ (k - l))
-
-let substractionInDomainNat #k #l a b = 
   lemma_mod_sub_distr a (l * pow2 256) prime;
   lemma_mod_add_distr (-l * pow2 256) (k * pow2 256) prime
-
-
-let substractionInDomain2Nat a b = 
-  let k = fromDomain_ a in 
-  let l = fromDomain_ b in 
-  lemmaFromDomainToDomain a;
-  lemmaFromDomainToDomain b;
-  substractionInDomainNat #k #l a b
 
 
 val lemmaDistributivityInDomain: a: int -> b: int -> Lemma (toDomain_ (a * (b % prime) % prime) = toDomain_ (a * b % prime))
