code/experimental/P256/Hacl.Impl.P256.LowLevel.fst
@@ -172,7 +172,7 @@ let p256_add arg1 arg2 out =
     lemma_t_computation t;
     reduction_prime256_2prime256_with_carry_impl t out out;
   let h2 = ST.get() in 
-    additionInDomain2Nat (as_nat h0 arg1) (as_nat h0 arg2);
+    additionInDomain (as_nat h0 arg1) (as_nat h0 arg2);
     inDomain_mod_is_not_mod (fromDomain_ (as_nat h0 arg1) + fromDomain_ (as_nat h0 arg2))
     (* lemma_eq_funct (as_seq h2 out) (felem_add_seq (as_seq h0 arg1) (as_seq h0 arg2)) *)
 
@@ -191,7 +191,7 @@ let p256_double arg1 out =
   lemma_t_computation t;
   reduction_prime256_2prime256_with_carry_impl t out out;
 
-  additionInDomain2Nat (as_nat h0 arg1) (as_nat h0 arg1);
+  additionInDomain (as_nat h0 arg1) (as_nat h0 arg1);
   inDomain_mod_is_not_mod (fromDomain_ (as_nat h0 arg1) + fromDomain_ (as_nat h0 arg1))
 
 (* to check *)
@@ -230,7 +230,7 @@ let p256_sub arg1 arg2 out =
             as_nat h2 out == (as_nat h0 arg1 - as_nat h0 arg2) % prime256
 	  end);
 
-    substractionInDomain2Nat (felem_seq_as_nat (as_seq h0 arg1)) (felem_seq_as_nat (as_seq h0 arg2));
+    substractionInDomain (felem_seq_as_nat (as_seq h0 arg1)) (felem_seq_as_nat (as_seq h0 arg2));
     inDomain_mod_is_not_mod (fromDomain_ (felem_seq_as_nat (as_seq h0 arg1)) - fromDomain_ (felem_seq_as_nat (as_seq h0 arg2)))
     (* lemma_eq_funct (as_seq h2 out) (felem_sub_seq (as_seq h0 arg1) (as_seq h0 arg2)) *)
     
