code/experimental/P256/Hacl.Spec.P256.MontgomeryMultiplication.fsti
@@ -4,23 +4,16 @@ open FStar.Math.Lemmas
 open FStar.Math.Lib
 open FStar.Mul
 
-open FStar.HyperStack.All
-open FStar.HyperStack
-open FStar.HyperStack.ST
-module ST = FStar.HyperStack.ST
-
 open Hacl.Spec.P256.Lemmas
 open Hacl.Spec.P256.Definitions
 open Hacl.Spec.P256.Core
 open Hacl.Spec.P256.Basic
 
 open Lib.IntTypes
-open Lib.Buffer
-open Lib.Sequence
 
 
 noextract
-val fromDomain_: a: int -> Tot (r: nat (*{ r = a * modp_inv2 (pow2 256) % prime256}*))
+val fromDomain_: a: int -> Tot nat
 
 noextract
 val fromDomainPoint: a: tuple3 nat nat nat -> Tot (r: tuple3 nat nat nat 
@@ -33,22 +26,19 @@ val fromDomainPoint: a: tuple3 nat nat nat -> Tot (r: tuple3 nat nat nat
 
 
 noextract
-val toDomain_: a: int -> Tot (r: nat (*{r =  a * pow2 256 % prime256}*))
+val toDomain_: a: int -> Tot nat
 
 val lemmaFromDomain: a: int -> Lemma (fromDomain_ (a) == a * modp_inv2 (pow2 256) % prime256)
 
 val lemmaToDomain: a: int -> Lemma (toDomain_(a) == a * (pow2 256) % prime256)
 
-val lemmaToDomainAndBackIsTheSame: a: nat { a < prime256} -> Lemma (fromDomain_ (toDomain_ a) == a)
+val lemmaToDomainAndBackIsTheSame: a: nat {a < prime256} -> Lemma (fromDomain_ (toDomain_ a) == a)
   [SMTPat (fromDomain_ (toDomain_ a))]
 
 val lemmaFromDomainToDomain: a: nat { a < prime256} -> Lemma (toDomain_ (fromDomain_ a) == a)
 
-
 val lemmaFromDomainToDomainModuloPrime: a: int -> Lemma (a % prime256 == fromDomain_(toDomain_ a))
 
-
-(* the lemma shows the equivalence between toDomain(a:nat) and toDomain(a % prime256) *)
 val inDomain_mod_is_not_mod: a: int -> Lemma (toDomain_ a == toDomain_ (a % prime256))
 
 val multiplicationInDomainNat: #k: nat -> #l: nat ->
@@ -58,12 +48,9 @@ val multiplicationInDomainNat: #k: nat -> #l: nat ->
     let multResult = a * b * modp_inv2_prime (pow2 256) prime256 % prime256 in 
     multResult == toDomain_ (k * l))
 
-val additionInDomain2Nat: a: nat {a < prime256} -> b: nat {b < prime256} -> Lemma 
-  (
-    let result = (a + b) % prime256 in 
-    result = toDomain_ (fromDomain_ a + fromDomain_ b)
-  )
+val additionInDomain: a: nat {a < prime256} -> b: nat {b < prime256} -> Lemma 
+  ((a + b) % prime256 == toDomain_ (fromDomain_ a + fromDomain_ b))
   
-val substractionInDomain2Nat: a: nat {a < prime256} -> b: nat { b < prime256} -> Lemma 
+val substractionInDomain: a: nat {a < prime256} -> b: nat { b < prime256} -> Lemma 
   ((a - b) % prime256 == toDomain_ (fromDomain_ a - fromDomain_ b))
   
